memset_spec init for forward_call

spec_streebog_init.v
@@ -8,6 +8,7 @@ Require Import functional_spec.
 Import ListNotations.
 
 
+
 (* void *shash_desc_ctx(struct shash_desc *desc)
 {
 	return desc->__ctx;
@@ -19,6 +20,28 @@ Definition t_streebog_state := Tstruct _streebog_state noattr.
 Definition t_crypto_shash := Tstruct _crypto_shash noattr.
 
 Definition shash_desc_ctx_spec :=
+  DECLARE _shash_desc_ctx
+  WITH descp: val
+  PRE [ tptr t_shash_desc ]
+    PROP (isptr descp)
+    PARAMS (descp)
+    SEP ()
+  POST [ tptr tvoid ]
+    PROP ()
+    RETURN (offset_val (sizeof t_shash_desc) descp)
+    SEP ().
+
+Lemma body_shash_desc_ctx :
+  semax_body Vprog [] f_shash_desc_ctx shash_desc_ctx_spec.
+Proof.
+  start_function.
+  forward.
+Qed.
+
+
+
+
+(* Definition shash_desc_ctx_spec :=
   DECLARE _shash_desc_ctx
   WITH sh : share, desc : val, ctx : val, tfm : val, ctx_content : block512 
   PRE [ tptr t_shash_desc]
@@ -47,7 +70,7 @@ Proof.
   entailer!.
   Compute sizeof (tptr tvoid).
 
-Admitted.
+Admitted. *)
 
 (*
 static int streebog_init(struct shash_desc *desc)
@@ -69,11 +92,26 @@ static int streebog_init(struct shash_desc *desc)
 
 Definition streebog_init_spec := 
   DECLARE _streebog_init 
-  WITH sh : share, desc : val, tfm : val, ctx : val, digest_size : Z, ctx_content : block512,
-            hash_content : block512, h_content : block512,
-            N_content : block512, Sigma_content : block512
-
+  WITH sh : share, desc : val, tfm : val
   PRE [tptr t_shash_desc]
+  PROP(writable_share sh;
+        isptr desc;
+        isptr tfm)
+  PARAMS (desc)
+  SEP (field_at sh t_shash_desc (DOT _tfm) tfm desc;
+        data_at_ sh t_streebog_state (offset_val (sizeof t_shash_desc) desc))
+
+  POST [ tint ]
+  PROP()
+  RETURN (Vint Int.zero)
+  SEP ( field_at sh t_shash_desc (DOT _tfm) tfm desc;
+        data_at_ sh t_streebog_state (offset_val (sizeof t_shash_desc) desc);
+        field_at sh t_streebog_state (DOT _h) (map Vlong (block512_to_int64s Vec512.zero)) (offset_val (sizeof t_shash_desc) desc) * 
+        field_at sh t_streebog_state (DOT _N) (map Vlong (block512_to_int64s Vec512.zero)) (offset_val (sizeof t_shash_desc) desc) * 
+        field_at sh t_streebog_state (DOT _Sigma) (map Vlong (block512_to_int64s Vec512.zero)) (offset_val (sizeof t_shash_desc) desc) * 
+        field_at sh t_streebog_state (DOT _hash) (map Vlong (block512_to_int64s Vec512.zero)) (offset_val (sizeof t_shash_desc) desc)).
+
+  (* PRE [tptr t_shash_desc]
     PROP(writable_share sh; digest_size = 64;
          Zlength (block512_to_int64s hash_content) = 8;
          Zlength (block512_to_int64s h_content) = 8;
@@ -87,8 +125,8 @@ Definition streebog_init_spec :=
              (map Vlong (block512_to_int64s h_content)) ctx * field_at sh t_streebog_state (DOT _N)
              (map Vlong (block512_to_int64s N_content)) ctx * field_at sh t_streebog_state (DOT _Sigma)
              (map Vlong (block512_to_int64s Sigma_content)) ctx * field_at sh t_streebog_state (DOT _hash)
-             (map Vlong (block512_to_int64s hash_content)) ctx)
-  POST [ tint ]
+             (map Vlong (block512_to_int64s hash_content)) ctx) *)
+  (* POST [ tint ]
     PROP()
     RETURN (Vint Int.zero)
     SEP ( field_at sh t_shash_desc (DOT ___ctx) (map Vlong (block512_to_int64s ctx_content)) desc * 
@@ -98,9 +136,19 @@ Definition streebog_init_spec :=
              (map Vlong (block512_to_int64s Vec512.zero)) ctx * field_at sh t_streebog_state (DOT _N)
              (map Vlong (block512_to_int64s Vec512.zero)) ctx * field_at sh t_streebog_state (DOT _Sigma)
              (map Vlong (block512_to_int64s Vec512.zero)) ctx * field_at sh t_streebog_state (DOT _hash)
-             (map Vlong (block512_to_int64s Vec512.zero)) ctx).
+             (map Vlong (block512_to_int64s Vec512.zero)) ctx). *)
 
-
+Definition memset_spec :=
+  DECLARE _memset
+   WITH sh : share, p: val, n: Z, c: int
+   PRE [ 1%positive OF tptr tvoid, 2%positive OF tint, 3%positive OF tuint ]
+       PROP (writable_share sh; 0 <= n <= Int.max_unsigned)
+       LOCAL (temp 1%positive p; temp 2%positive (Vint c);
+                   temp 3%positive (Vint (Int.repr n)))
+       SEP (memory_block sh n p)
+    POST [ tptr tvoid ]
+       PROP() LOCAL(temp ret_temp p)
+       SEP(data_at sh (tarray tuchar n) (repeat (Vint c) (Z.to_nat n)) p).
 
 
 Definition Gprog : funspecs :=
@@ -112,7 +160,12 @@ Lemma body_streebog_init :
 Proof.
   start_function.
   Intros.
-  forward_call(sh, desc, ctx, tfm, ctx_content).
+  forward_call(desc).
+  forward.
+  hint.
+  Check memset.
+  (* forward_call (sh, offset_val (sizeof t_shash_desc) desc, sizeof t_streebog_state). *)
+
 
 Qed.
 
